Make paper example fit the paper better.

examples/paper_examples.c
@@ -3,66 +3,64 @@
 #include <refinedc.h>
 #include <spinlock.h>
 
-struct [[rc::refined_by("nlen : nat")]] alloc_data {
-  [[rc::field("nlen @ int<size_t>")]]
-  size_t len;
-  [[rc::field("&own<uninit<{ly_set_size u8 nlen}>>")]]
-  unsigned char *buffer;
+//@rc::inlined
+//@Notation "P ? l : r" :=
+//@  (if bool_decide P then l else r)
+//@  (at level 100, l at next level, r at next level).
+//@
+//@Close Scope Z.
+//@
+//@Definition byte_layout : nat → layout := ly_set_size u8.
+//@Coercion byte_layout : nat >-> layout.
+//@rc::end
+
+//// Example of Section 2.1 //////////////////////////////////////////////////
+
+struct [[rc::refined_by("a : nat")]] mem_t {
+  [[rc::field("a @ int<size_t>")]] size_t len;
+  [[rc::field("&own<uninit<a>>")]] unsigned char *buffer;
 };
-[[rc::parameters("nlen : nat", "nsize : nat", "p : loc")]]
-[[rc::args("p @ &own<nlen @ alloc_data>", "nsize @ int<size_t>")]]
-[[rc::returns("{nsize <= nlen} @ optional<&own<uninit<{ly_set_size u8 nsize}>>, null>")]]
-[[rc::ensures("p @ &own<{if bool_decide(nsize <= nlen) then (nlen - nsize)%nat else nlen} @ alloc_data>")]]
-void *alloc(struct alloc_data *d, size_t size) {
-  if(size > d->len) {
-    return NULL;
-  }
+
+[[rc::parameters("a : nat", "n : nat", "p : loc")]]
+[[rc::args   ("p @ &own<a @ mem_t>", "n @ int<size_t>")]]
+[[rc::returns("{n ≤ a} @ optional<&own<uninit<n>>, null>")]]
+[[rc::ensures("p @ &own<{n ≤ a ? a - n : a} @ mem_t>")]]
+void *alloc(struct mem_t *d, size_t size) {
+  if(size > d->len) return NULL;
   d->len -= size;
   return d->buffer + d->len;
 }
 
-[[rc::parameters("lid : lock_id")]]
-[[rc::global("spinlock<lid>")]]
-struct spinlock lock;
+//// Example of Section 2.2 //////////////////////////////////////////////////
 
-[[rc::parameters("lid : lock_id")]]
-[[rc::global("spinlocked<lid, {\"data\"}, alloc_data>")]]
-struct alloc_data data;
-
-[[rc::parameters("lid : lock_id", "nsize : nat")]]
-[[rc::args      ("nsize @ int<size_t>")]]
-[[rc::requires  ("[initialized \"lock\" lid]", "[initialized \"data\" lid]")]]
-[[rc::returns   ("optional<&own<uninit<{ly_set_size u8 nsize}>>, null>")]]
-void *thread_safe_alloc(size_t size) {
-  sl_lock(&lock);
-  rc_unlock(data);
-  void *ret = alloc(&data, size);
-  sl_unlock(&lock);
-  return ret;
-}
-
+// In the paper this example is simplified to ignore memory alignment.
+// For the actual example we work on multisets of layouts, not nat.
 
 typedef struct
 [[rc::refined_by("s: {gmultiset layout}")]]
 [[rc::ptr_type("chunks_t : {s ≠ ∅} @ optional<&own<...>, null>")]]
-[[rc::exists("ly : layout", "tail : {gmultiset layout}")]]
-[[rc::size("ly")]]
-[[rc::constraints("{s = {[ly]} ⊎ tail}", "{∀ k, k ∈ tail → ly.(ly_size) ≤ k.(ly_size)}")]]
+[[rc::exists  ("ly : layout", "tail : {gmultiset layout}")]]
+[[rc::size    ("ly")]]
+[[rc::constraints("{s = {[ly]} ⊎ tail}",
+                  "{∀ k, k ∈ tail → ly.(ly_size) ≤ k.(ly_size)}")]]
 chunk {
   [[rc::field("{ly.(ly_size)} @ int<size_t>")]] size_t size;
   [[rc::field("tail @ chunks_t")]] struct chunk* next;
 }* chunks_t;
 
 [[rc::parameters("s : {gmultiset layout}", "p : loc", "ly : layout")]]
-[[rc::args("p @ &own<s @ chunks_t>", "&own<uninit<ly>>", "{ly.(ly_size)} @ int<size_t>")]]
-[[rc::requires("{layout_of struct_chunk ⊑ ly}")]]
-[[rc::ensures("p @ &own<{{[ly]} ⊎ s} @ chunks_t>")]]
-[[rc::tactics("all: multiset_solver.")]]
+[[rc::args      ("p @ &own<s @ chunks_t>", "&own<uninit<ly>>",
+                 "{ly.(ly_size)} @ int<size_t>")]]
+[[rc::requires  ("{layout_of struct_chunk ⊑ ly}")]]
+[[rc::ensures   ("p @ &own<{{[ly]} ⊎ s} @ chunks_t>")]]
+[[rc::tactics   ("all: multiset_solver.")]]
 void free(chunks_t* list, void *data, size_t size) {
   chunks_t *cur = list;
-  [[rc::exists("cp : loc", "cs : {gmultiset layout}")]]
+  [[rc::exists  ("cp : loc", "cs : {gmultiset layout}")]]
   [[rc::inv_vars("cur : cp @ &own<cs @ chunks_t>")]]
-  [[rc::inv_vars("list : p @ &own<wand<{cp ◁ₗ ({[ly]} ⊎ cs) @ chunks_t}, {{[ly]} ⊎ s} @ chunks_t>>")]]
+  [[rc::inv_vars("list : p @ &own<"
+                   "wand<{cp ◁ₗ ({[ly]} ⊎ cs) @ chunks_t}, "
+                   "{{[ly]} ⊎ s} @ chunks_t>>")]]
   while(*cur != NULL) {
     if(size <= (*cur)->size) break;
     cur = &(*cur)->next;
@@ -73,10 +71,35 @@ void free(chunks_t* list, void *data, size_t size) {
   *cur = entry;
 }
 
-/** Testing the thread-safety of thread_safe alloc */
+//// Example given in appendix ///////////////////////////////////////////////
 
-// RefinedC does not have forking built-in at the moment, so we axiomatize it using the following [fork] function
+[[rc::parameters("lid : lock_id")]]
+[[rc::global("spinlock<lid>")]]
+struct spinlock lock;
+
+[[rc::parameters("lid : lock_id")]]
+[[rc::global("spinlocked<lid, {\"data\"}, mem_t>")]]
+struct mem_t data;
+
+[[rc::parameters("lid : lock_id", "n : nat")]]
+[[rc::args      ("n @ int<size_t>")]]
+[[rc::requires  ("[initialized \"lock\" lid]", "[initialized \"data\" lid]")]]
+[[rc::returns   ("optional<&own<uninit<n>>, null>")]]
+void *thread_safe_alloc(size_t size) {
+  sl_lock(&lock);
+  rc_unlock(data);
+  void *ret = alloc(&data, size);
+  sl_unlock(&lock);
+  return ret;
+}
+
+//// Testing thread-safety of thread_safe alloc //////////////////////////////
+
+// RefinedC does not have forking built-in at the moment.
+// We axiomatize it using the following [fork] function.
+
 typedef void (*fork_fun)(void *);
+
 [[rc::parameters("ty : type", "P : {iProp Σ}")]]
 [[rc::args("function_ptr<{fn(∀ () : (); &own ty; P) → ∃ () : (), void; True}>", "&own<ty>")]]
 [[rc::requires("[P]")]]
