examples/proofs/paper_examples/generated_code.v
@@ -7,148 +7,147 @@ Set Default Proof Using "Type".
 (* Generated from [examples/paper_examples.c]. *)
 Section code.
   Definition file_0 : string := "examples/paper_examples.c".
-  Definition loc_2 : location_info := LocationInfo file_0 17 2 19 3.
-  Definition loc_3 : location_info := LocationInfo file_0 20 2 20 17.
-  Definition loc_4 : location_info := LocationInfo file_0 21 2 21 28.
-  Definition loc_5 : location_info := LocationInfo file_0 21 9 21 27.
-  Definition loc_6 : location_info := LocationInfo file_0 21 9 21 18.
-  Definition loc_7 : location_info := LocationInfo file_0 21 9 21 18.
-  Definition loc_8 : location_info := LocationInfo file_0 21 9 21 10.
-  Definition loc_9 : location_info := LocationInfo file_0 21 9 21 10.
-  Definition loc_10 : location_info := LocationInfo file_0 21 21 21 27.
-  Definition loc_11 : location_info := LocationInfo file_0 21 21 21 27.
-  Definition loc_12 : location_info := LocationInfo file_0 21 21 21 22.
-  Definition loc_13 : location_info := LocationInfo file_0 21 21 21 22.
-  Definition loc_14 : location_info := LocationInfo file_0 20 2 20 8.
-  Definition loc_15 : location_info := LocationInfo file_0 20 2 20 3.
-  Definition loc_16 : location_info := LocationInfo file_0 20 2 20 3.
-  Definition loc_17 : location_info := LocationInfo file_0 20 2 20 16.
-  Definition loc_18 : location_info := LocationInfo file_0 20 2 20 8.
-  Definition loc_19 : location_info := LocationInfo file_0 20 2 20 8.
-  Definition loc_20 : location_info := LocationInfo file_0 20 2 20 3.
-  Definition loc_21 : location_info := LocationInfo file_0 20 2 20 3.
-  Definition loc_22 : location_info := LocationInfo file_0 20 12 20 16.
-  Definition loc_23 : location_info := LocationInfo file_0 20 12 20 16.
-  Definition loc_24 : location_info := LocationInfo file_0 17 20 19 3.
-  Definition loc_25 : location_info := LocationInfo file_0 18 4 18 26.
-  Definition loc_26 : location_info := LocationInfo file_0 18 11 18 25.
-  Definition loc_28 : location_info := LocationInfo file_0 17 5 17 18.
-  Definition loc_29 : location_info := LocationInfo file_0 17 5 17 9.
-  Definition loc_30 : location_info := LocationInfo file_0 17 5 17 9.
-  Definition loc_31 : location_info := LocationInfo file_0 17 12 17 18.
-  Definition loc_32 : location_info := LocationInfo file_0 17 12 17 18.
-  Definition loc_33 : location_info := LocationInfo file_0 17 12 17 13.
-  Definition loc_34 : location_info := LocationInfo file_0 17 12 17 13.
-  Definition loc_37 : location_info := LocationInfo file_0 37 2 37 17.
-  Definition loc_38 : location_info := LocationInfo file_0 38 2 38 35.
-  Definition loc_39 : location_info := LocationInfo file_0 38 35 38 3.
-  Definition loc_40 : location_info := LocationInfo file_0 39 2 39 33.
-  Definition loc_41 : location_info := LocationInfo file_0 40 2 40 19.
-  Definition loc_42 : location_info := LocationInfo file_0 41 2 41 13.
-  Definition loc_43 : location_info := LocationInfo file_0 41 9 41 12.
-  Definition loc_44 : location_info := LocationInfo file_0 41 9 41 12.
-  Definition loc_45 : location_info := LocationInfo file_0 40 2 40 11.
-  Definition loc_46 : location_info := LocationInfo file_0 40 2 40 11.
-  Definition loc_47 : location_info := LocationInfo file_0 40 12 40 17.
-  Definition loc_48 : location_info := LocationInfo file_0 40 13 40 17.
-  Definition loc_49 : location_info := LocationInfo file_0 39 14 39 32.
-  Definition loc_50 : location_info := LocationInfo file_0 39 14 39 19.
-  Definition loc_51 : location_info := LocationInfo file_0 39 14 39 19.
-  Definition loc_52 : location_info := LocationInfo file_0 39 20 39 25.
-  Definition loc_53 : location_info := LocationInfo file_0 39 21 39 25.
-  Definition loc_54 : location_info := LocationInfo file_0 39 27 39 31.
-  Definition loc_55 : location_info := LocationInfo file_0 39 27 39 31.
-  Definition loc_58 : location_info := LocationInfo file_0 38 27 38 34.
-  Definition loc_59 : location_info := LocationInfo file_0 38 28 38 34.
-  Definition loc_60 : location_info := LocationInfo file_0 37 2 37 9.
-  Definition loc_61 : location_info := LocationInfo file_0 37 2 37 9.
-  Definition loc_62 : location_info := LocationInfo file_0 37 10 37 15.
-  Definition loc_63 : location_info := LocationInfo file_0 37 11 37 15.
-  Definition loc_66 : location_info := LocationInfo file_0 62 2 62 23.
-  Definition loc_67 : location_info := LocationInfo file_0 66 2 69 3.
-  Definition loc_68 : location_info := LocationInfo file_0 70 2 70 24.
-  Definition loc_69 : location_info := LocationInfo file_0 71 2 71 21.
-  Definition loc_70 : location_info := LocationInfo file_0 72 2 72 21.
-  Definition loc_71 : location_info := LocationInfo file_0 73 2 73 15.
-  Definition loc_72 : location_info := LocationInfo file_0 73 2 73 6.
-  Definition loc_73 : location_info := LocationInfo file_0 73 3 73 6.
-  Definition loc_74 : location_info := LocationInfo file_0 73 3 73 6.
-  Definition loc_75 : location_info := LocationInfo file_0 73 9 73 14.
-  Definition loc_76 : location_info := LocationInfo file_0 73 9 73 14.
-  Definition loc_77 : location_info := LocationInfo file_0 72 2 72 13.
-  Definition loc_78 : location_info := LocationInfo file_0 72 2 72 7.
-  Definition loc_79 : location_info := LocationInfo file_0 72 2 72 7.
-  Definition loc_80 : location_info := LocationInfo file_0 72 16 72 20.
-  Definition loc_81 : location_info := LocationInfo file_0 72 16 72 20.
-  Definition loc_82 : location_info := LocationInfo file_0 72 17 72 20.
-  Definition loc_83 : location_info := LocationInfo file_0 72 17 72 20.
-  Definition loc_84 : location_info := LocationInfo file_0 71 2 71 13.
-  Definition loc_85 : location_info := LocationInfo file_0 71 2 71 7.
-  Definition loc_86 : location_info := LocationInfo file_0 71 2 71 7.
-  Definition loc_87 : location_info := LocationInfo file_0 71 16 71 20.
-  Definition loc_88 : location_info := LocationInfo file_0 71 16 71 20.
-  Definition loc_89 : location_info := LocationInfo file_0 70 19 70 23.
-  Definition loc_90 : location_info := LocationInfo file_0 70 19 70 23.
-  Definition loc_93 : location_info := LocationInfo file_0 66 2 69 3.
-  Definition loc_94 : location_info := LocationInfo file_0 66 32 69 3.
-  Definition loc_95 : location_info := LocationInfo file_0 67 4 67 35.
-  Definition loc_96 : location_info := LocationInfo file_0 68 4 68 24.
-  Definition loc_97 : location_info := LocationInfo file_0 66 2 69 3.
-  Definition loc_98 : location_info := LocationInfo file_0 66 2 69 3.
-  Definition loc_99 : location_info := LocationInfo file_0 68 4 68 7.
-  Definition loc_100 : location_info := LocationInfo file_0 68 10 68 23.
-  Definition loc_101 : location_info := LocationInfo file_0 68 11 68 23.
-  Definition loc_102 : location_info := LocationInfo file_0 68 11 68 17.
-  Definition loc_103 : location_info := LocationInfo file_0 68 11 68 17.
-  Definition loc_104 : location_info := LocationInfo file_0 68 13 68 16.
-  Definition loc_105 : location_info := LocationInfo file_0 68 13 68 16.
-  Definition loc_106 : location_info := LocationInfo file_0 67 29 67 35.
-  Definition loc_108 : location_info := LocationInfo file_0 67 7 67 27.
-  Definition loc_109 : location_info := LocationInfo file_0 67 7 67 11.
-  Definition loc_110 : location_info := LocationInfo file_0 67 7 67 11.
-  Definition loc_111 : location_info := LocationInfo file_0 67 15 67 27.
-  Definition loc_112 : location_info := LocationInfo file_0 67 15 67 27.
-  Definition loc_113 : location_info := LocationInfo file_0 67 15 67 21.
-  Definition loc_114 : location_info := LocationInfo file_0 67 15 67 21.
-  Definition loc_115 : location_info := LocationInfo file_0 67 17 67 20.
-  Definition loc_116 : location_info := LocationInfo file_0 67 17 67 20.
-  Definition loc_117 : location_info := LocationInfo file_0 66 8 66 30.
-  Definition loc_118 : location_info := LocationInfo file_0 66 8 66 12.
-  Definition loc_119 : location_info := LocationInfo file_0 66 8 66 12.
-  Definition loc_120 : location_info := LocationInfo file_0 66 9 66 12.
-  Definition loc_121 : location_info := LocationInfo file_0 66 9 66 12.
-  Definition loc_122 : location_info := LocationInfo file_0 66 16 66 30.
-  Definition loc_123 : location_info := LocationInfo file_0 62 18 62 22.
-  Definition loc_124 : location_info := LocationInfo file_0 62 18 62 22.
-  Definition loc_129 : location_info := LocationInfo file_0 84 2 84 10.
-  Definition loc_130 : location_info := LocationInfo file_0 84 2 84 4.
-  Definition loc_131 : location_info := LocationInfo file_0 84 2 84 4.
-  Definition loc_132 : location_info := LocationInfo file_0 84 2 84 4.
-  Definition loc_133 : location_info := LocationInfo file_0 84 5 84 8.
-  Definition loc_134 : location_info := LocationInfo file_0 84 5 84 8.
-  Definition loc_137 : location_info := LocationInfo file_0 90 2 90 24.
-  Definition loc_138 : location_info := LocationInfo file_0 91 2 91 30.
-  Definition loc_139 : location_info := LocationInfo file_0 91 2 91 19.
-  Definition loc_140 : location_info := LocationInfo file_0 91 2 91 19.
-  Definition loc_141 : location_info := LocationInfo file_0 91 20 91 28.
-  Definition loc_142 : location_info := LocationInfo file_0 91 20 91 28.
-  Definition loc_143 : location_info := LocationInfo file_0 91 21 91 28.
-  Definition loc_144 : location_info := LocationInfo file_0 91 21 91 28.
-  Definition loc_145 : location_info := LocationInfo file_0 90 20 90 23.
-  Definition loc_146 : location_info := LocationInfo file_0 90 20 90 23.
-  Definition loc_151 : location_info := LocationInfo file_0 100 2 100 12.
-  Definition loc_152 : location_info := LocationInfo file_0 101 2 101 47.
-  Definition loc_153 : location_info := LocationInfo file_0 102 2 102 23.
-  Definition loc_154 : location_info := LocationInfo file_0 102 2 102 19.
-  Definition loc_155 : location_info := LocationInfo file_0 102 2 102 19.
-  Definition loc_156 : location_info := LocationInfo file_0 102 20 102 21.
-  Definition loc_157 : location_info := LocationInfo file_0 101 2 101 6.
-  Definition loc_158 : location_info := LocationInfo file_0 101 2 101 6.
-  Definition loc_159 : location_info := LocationInfo file_0 101 7 101 37.
-  Definition loc_160 : location_info := LocationInfo file_0 101 39 101 45.
-  Definition loc_161 : location_info := LocationInfo file_0 101 40 101 45.
-  Definition loc_162 : location_info := LocationInfo file_0 100 2 100 7.
-  Definition loc_163 : location_info := LocationInfo file_0 100 10 100 11.
+  Definition loc_2 : location_info := LocationInfo file_0 29 2 29 42.
+  Definition loc_3 : location_info := LocationInfo file_0 30 2 30 17.
+  Definition loc_4 : location_info := LocationInfo file_0 31 2 31 28.
+  Definition loc_5 : location_info := LocationInfo file_0 31 9 31 27.
+  Definition loc_6 : location_info := LocationInfo file_0 31 9 31 18.
+  Definition loc_7 : location_info := LocationInfo file_0 31 9 31 18.
+  Definition loc_8 : location_info := LocationInfo file_0 31 9 31 10.
+  Definition loc_9 : location_info := LocationInfo file_0 31 9 31 10.
+  Definition loc_10 : location_info := LocationInfo file_0 31 21 31 27.
+  Definition loc_11 : location_info := LocationInfo file_0 31 21 31 27.
+  Definition loc_12 : location_info := LocationInfo file_0 31 21 31 22.
+  Definition loc_13 : location_info := LocationInfo file_0 31 21 31 22.
+  Definition loc_14 : location_info := LocationInfo file_0 30 2 30 8.
+  Definition loc_15 : location_info := LocationInfo file_0 30 2 30 3.
+  Definition loc_16 : location_info := LocationInfo file_0 30 2 30 3.
+  Definition loc_17 : location_info := LocationInfo file_0 30 2 30 16.
+  Definition loc_18 : location_info := LocationInfo file_0 30 2 30 8.
+  Definition loc_19 : location_info := LocationInfo file_0 30 2 30 8.
+  Definition loc_20 : location_info := LocationInfo file_0 30 2 30 3.
+  Definition loc_21 : location_info := LocationInfo file_0 30 2 30 3.
+  Definition loc_22 : location_info := LocationInfo file_0 30 12 30 16.
+  Definition loc_23 : location_info := LocationInfo file_0 30 12 30 16.
+  Definition loc_24 : location_info := LocationInfo file_0 29 20 29 42.
+  Definition loc_25 : location_info := LocationInfo file_0 29 27 29 41.
+  Definition loc_27 : location_info := LocationInfo file_0 29 5 29 18.
+  Definition loc_28 : location_info := LocationInfo file_0 29 5 29 9.
+  Definition loc_29 : location_info := LocationInfo file_0 29 5 29 9.
+  Definition loc_30 : location_info := LocationInfo file_0 29 12 29 18.
+  Definition loc_31 : location_info := LocationInfo file_0 29 12 29 18.
+  Definition loc_32 : location_info := LocationInfo file_0 29 12 29 13.
+  Definition loc_33 : location_info := LocationInfo file_0 29 12 29 13.
+  Definition loc_36 : location_info := LocationInfo file_0 58 2 58 23.
+  Definition loc_37 : location_info := LocationInfo file_0 64 2 67 3.
+  Definition loc_38 : location_info := LocationInfo file_0 68 2 68 24.
+  Definition loc_39 : location_info := LocationInfo file_0 69 2 69 21.
+  Definition loc_40 : location_info := LocationInfo file_0 70 2 70 21.
+  Definition loc_41 : location_info := LocationInfo file_0 71 2 71 15.
+  Definition loc_42 : location_info := LocationInfo file_0 71 2 71 6.
+  Definition loc_43 : location_info := LocationInfo file_0 71 3 71 6.
+  Definition loc_44 : location_info := LocationInfo file_0 71 3 71 6.
+  Definition loc_45 : location_info := LocationInfo file_0 71 9 71 14.
+  Definition loc_46 : location_info := LocationInfo file_0 71 9 71 14.
+  Definition loc_47 : location_info := LocationInfo file_0 70 2 70 13.
+  Definition loc_48 : location_info := LocationInfo file_0 70 2 70 7.
+  Definition loc_49 : location_info := LocationInfo file_0 70 2 70 7.
+  Definition loc_50 : location_info := LocationInfo file_0 70 16 70 20.
+  Definition loc_51 : location_info := LocationInfo file_0 70 16 70 20.
+  Definition loc_52 : location_info := LocationInfo file_0 70 17 70 20.
+  Definition loc_53 : location_info := LocationInfo file_0 70 17 70 20.
+  Definition loc_54 : location_info := LocationInfo file_0 69 2 69 13.
+  Definition loc_55 : location_info := LocationInfo file_0 69 2 69 7.
+  Definition loc_56 : location_info := LocationInfo file_0 69 2 69 7.
+  Definition loc_57 : location_info := LocationInfo file_0 69 16 69 20.
+  Definition loc_58 : location_info := LocationInfo file_0 69 16 69 20.
+  Definition loc_59 : location_info := LocationInfo file_0 68 19 68 23.
+  Definition loc_60 : location_info := LocationInfo file_0 68 19 68 23.
+  Definition loc_63 : location_info := LocationInfo file_0 64 2 67 3.
+  Definition loc_64 : location_info := LocationInfo file_0 64 32 67 3.
+  Definition loc_65 : location_info := LocationInfo file_0 65 4 65 35.
+  Definition loc_66 : location_info := LocationInfo file_0 66 4 66 24.
+  Definition loc_67 : location_info := LocationInfo file_0 64 2 67 3.
+  Definition loc_68 : location_info := LocationInfo file_0 64 2 67 3.
+  Definition loc_69 : location_info := LocationInfo file_0 66 4 66 7.
+  Definition loc_70 : location_info := LocationInfo file_0 66 10 66 23.
+  Definition loc_71 : location_info := LocationInfo file_0 66 11 66 23.
+  Definition loc_72 : location_info := LocationInfo file_0 66 11 66 17.
+  Definition loc_73 : location_info := LocationInfo file_0 66 11 66 17.
+  Definition loc_74 : location_info := LocationInfo file_0 66 13 66 16.
+  Definition loc_75 : location_info := LocationInfo file_0 66 13 66 16.
+  Definition loc_76 : location_info := LocationInfo file_0 65 29 65 35.
+  Definition loc_78 : location_info := LocationInfo file_0 65 7 65 27.
+  Definition loc_79 : location_info := LocationInfo file_0 65 7 65 11.
+  Definition loc_80 : location_info := LocationInfo file_0 65 7 65 11.
+  Definition loc_81 : location_info := LocationInfo file_0 65 15 65 27.
+  Definition loc_82 : location_info := LocationInfo file_0 65 15 65 27.
+  Definition loc_83 : location_info := LocationInfo file_0 65 15 65 21.
+  Definition loc_84 : location_info := LocationInfo file_0 65 15 65 21.
+  Definition loc_85 : location_info := LocationInfo file_0 65 17 65 20.
+  Definition loc_86 : location_info := LocationInfo file_0 65 17 65 20.
+  Definition loc_87 : location_info := LocationInfo file_0 64 8 64 30.
+  Definition loc_88 : location_info := LocationInfo file_0 64 8 64 12.
+  Definition loc_89 : location_info := LocationInfo file_0 64 8 64 12.
+  Definition loc_90 : location_info := LocationInfo file_0 64 9 64 12.
+  Definition loc_91 : location_info := LocationInfo file_0 64 9 64 12.
+  Definition loc_92 : location_info := LocationInfo file_0 64 16 64 30.
+  Definition loc_93 : location_info := LocationInfo file_0 58 18 58 22.
+  Definition loc_94 : location_info := LocationInfo file_0 58 18 58 22.
+  Definition loc_99 : location_info := LocationInfo file_0 89 2 89 17.
+  Definition loc_100 : location_info := LocationInfo file_0 90 2 90 35.
+  Definition loc_101 : location_info := LocationInfo file_0 90 35 90 3.
+  Definition loc_102 : location_info := LocationInfo file_0 91 2 91 33.
+  Definition loc_103 : location_info := LocationInfo file_0 92 2 92 19.
+  Definition loc_104 : location_info := LocationInfo file_0 93 2 93 13.
+  Definition loc_105 : location_info := LocationInfo file_0 93 9 93 12.
+  Definition loc_106 : location_info := LocationInfo file_0 93 9 93 12.
+  Definition loc_107 : location_info := LocationInfo file_0 92 2 92 11.
+  Definition loc_108 : location_info := LocationInfo file_0 92 2 92 11.
+  Definition loc_109 : location_info := LocationInfo file_0 92 12 92 17.
+  Definition loc_110 : location_info := LocationInfo file_0 92 13 92 17.
+  Definition loc_111 : location_info := LocationInfo file_0 91 14 91 32.
+  Definition loc_112 : location_info := LocationInfo file_0 91 14 91 19.
+  Definition loc_113 : location_info := LocationInfo file_0 91 14 91 19.
+  Definition loc_114 : location_info := LocationInfo file_0 91 20 91 25.
+  Definition loc_115 : location_info := LocationInfo file_0 91 21 91 25.
+  Definition loc_116 : location_info := LocationInfo file_0 91 27 91 31.
+  Definition loc_117 : location_info := LocationInfo file_0 91 27 91 31.
+  Definition loc_120 : location_info := LocationInfo file_0 90 27 90 34.
+  Definition loc_121 : location_info := LocationInfo file_0 90 28 90 34.
+  Definition loc_122 : location_info := LocationInfo file_0 89 2 89 9.
+  Definition loc_123 : location_info := LocationInfo file_0 89 2 89 9.
+  Definition loc_124 : location_info := LocationInfo file_0 89 10 89 15.
+  Definition loc_125 : location_info := LocationInfo file_0 89 11 89 15.
+  Definition loc_128 : location_info := LocationInfo file_0 107 2 107 10.
+  Definition loc_129 : location_info := LocationInfo file_0 107 2 107 4.
+  Definition loc_130 : location_info := LocationInfo file_0 107 2 107 4.
+  Definition loc_131 : location_info := LocationInfo file_0 107 2 107 4.
+  Definition loc_132 : location_info := LocationInfo file_0 107 5 107 8.
+  Definition loc_133 : location_info := LocationInfo file_0 107 5 107 8.
+  Definition loc_136 : location_info := LocationInfo file_0 113 2 113 24.
+  Definition loc_137 : location_info := LocationInfo file_0 114 2 114 30.
+  Definition loc_138 : location_info := LocationInfo file_0 114 2 114 19.
+  Definition loc_139 : location_info := LocationInfo file_0 114 2 114 19.
+  Definition loc_140 : location_info := LocationInfo file_0 114 20 114 28.
+  Definition loc_141 : location_info := LocationInfo file_0 114 20 114 28.
+  Definition loc_142 : location_info := LocationInfo file_0 114 21 114 28.
+  Definition loc_143 : location_info := LocationInfo file_0 114 21 114 28.
+  Definition loc_144 : location_info := LocationInfo file_0 113 20 113 23.
+  Definition loc_145 : location_info := LocationInfo file_0 113 20 113 23.
+  Definition loc_150 : location_info := LocationInfo file_0 123 2 123 12.
+  Definition loc_151 : location_info := LocationInfo file_0 124 2 124 47.
+  Definition loc_152 : location_info := LocationInfo file_0 125 2 125 23.
+  Definition loc_153 : location_info := LocationInfo file_0 125 2 125 19.
+  Definition loc_154 : location_info := LocationInfo file_0 125 2 125 19.
+  Definition loc_155 : location_info := LocationInfo file_0 125 20 125 21.
+  Definition loc_156 : location_info := LocationInfo file_0 124 2 124 6.
+  Definition loc_157 : location_info := LocationInfo file_0 124 2 124 6.
+  Definition loc_158 : location_info := LocationInfo file_0 124 7 124 37.
+  Definition loc_159 : location_info := LocationInfo file_0 124 39 124 45.
+  Definition loc_160 : location_info := LocationInfo file_0 124 40 124 45.
+  Definition loc_161 : location_info := LocationInfo file_0 123 2 123 7.
+  Definition loc_162 : location_info := LocationInfo file_0 123 10 123 11.
 
   (* Definition of struct [atomic_flag]. *)
   Program Definition struct_atomic_flag := {|
@@ -166,8 +165,8 @@ Section code.
   |}.
   Solve Obligations with solve_struct_obligations.
 
-  (* Definition of struct [alloc_data]. *)
-  Program Definition struct_alloc_data := {|
+  (* Definition of struct [mem_t]. *)
+  Program Definition struct_mem_t := {|
     sl_members := [
       (Some "len", it_layout size_t);
       (Some "buffer", LPtr)
@@ -195,10 +194,10 @@ Section code.
     f_init := "#0";
     f_code := (
       <[ "#0" :=
-        locinfo: loc_28 ;
-        if: LocInfoE loc_28 (UnOp (CastOp $ IntOp bool_it) (IntOp i32) (LocInfoE loc_28 ((LocInfoE loc_29 (use{it_layout size_t} (LocInfoE loc_30 ("size")))) >{IntOp size_t, IntOp size_t} (LocInfoE loc_31 (use{it_layout size_t} (LocInfoE loc_32 ((LocInfoE loc_33 (!{LPtr} (LocInfoE loc_34 ("d")))) at{struct_alloc_data} "len")))))))
+        locinfo: loc_27 ;
+        if: LocInfoE loc_27 (UnOp (CastOp $ IntOp bool_it) (IntOp i32) (LocInfoE loc_27 ((LocInfoE loc_28 (use{it_layout size_t} (LocInfoE loc_29 ("size")))) >{IntOp size_t, IntOp size_t} (LocInfoE loc_30 (use{it_layout size_t} (LocInfoE loc_31 ((LocInfoE loc_32 (!{LPtr} (LocInfoE loc_33 ("d")))) at{struct_mem_t} "len")))))))
         then
-        locinfo: loc_25 ;
+        locinfo: loc_24 ;
           Goto "#2"
         else
         locinfo: loc_3 ;
@@ -206,49 +205,18 @@ Section code.
       ]> $
       <[ "#1" :=
         locinfo: loc_3 ;
-        LocInfoE loc_14 ((LocInfoE loc_15 (!{LPtr} (LocInfoE loc_16 ("d")))) at{struct_alloc_data} "len") <-{ it_layout size_t }
-          LocInfoE loc_17 ((LocInfoE loc_18 (use{it_layout size_t} (LocInfoE loc_19 ((LocInfoE loc_20 (!{LPtr} (LocInfoE loc_21 ("d")))) at{struct_alloc_data} "len")))) -{IntOp size_t, IntOp size_t} (LocInfoE loc_22 (use{it_layout size_t} (LocInfoE loc_23 ("size"))))) ;
+        LocInfoE loc_14 ((LocInfoE loc_15 (!{LPtr} (LocInfoE loc_16 ("d")))) at{struct_mem_t} "len") <-{ it_layout size_t }
+          LocInfoE loc_17 ((LocInfoE loc_18 (use{it_layout size_t} (LocInfoE loc_19 ((LocInfoE loc_20 (!{LPtr} (LocInfoE loc_21 ("d")))) at{struct_mem_t} "len")))) -{IntOp size_t, IntOp size_t} (LocInfoE loc_22 (use{it_layout size_t} (LocInfoE loc_23 ("size"))))) ;
         locinfo: loc_4 ;
-        Return (LocInfoE loc_5 ((LocInfoE loc_6 (use{LPtr} (LocInfoE loc_7 ((LocInfoE loc_8 (!{LPtr} (LocInfoE loc_9 ("d")))) at{struct_alloc_data} "buffer")))) at_offset{it_layout u8, PtrOp, IntOp size_t} (LocInfoE loc_10 (use{it_layout size_t} (LocInfoE loc_11 ((LocInfoE loc_12 (!{LPtr} (LocInfoE loc_13 ("d")))) at{struct_alloc_data} "len"))))))
+        Return (LocInfoE loc_5 ((LocInfoE loc_6 (use{LPtr} (LocInfoE loc_7 ((LocInfoE loc_8 (!{LPtr} (LocInfoE loc_9 ("d")))) at{struct_mem_t} "buffer")))) at_offset{it_layout u8, PtrOp, IntOp size_t} (LocInfoE loc_10 (use{it_layout size_t} (LocInfoE loc_11 ((LocInfoE loc_12 (!{LPtr} (LocInfoE loc_13 ("d")))) at{struct_mem_t} "len"))))))
       ]> $
       <[ "#2" :=
-        locinfo: loc_25 ;
-        Return (LocInfoE loc_26 (NULL))
+        locinfo: loc_24 ;
+        Return (LocInfoE loc_25 (NULL))
       ]> $
       <[ "#3" :=
         locinfo: loc_3 ;
         Goto "#1"
-      ]> $∅
-    )%E
-  |}.
-
-  (* Definition of function [thread_safe_alloc]. *)
-  Definition impl_thread_safe_alloc (data lock alloc sl_lock sl_unlock : loc): function := {|
-    f_args := [
-      ("size", it_layout size_t)
-    ];
-    f_local_vars := [
-      ("ret", LPtr)
-    ];
-    f_init := "#0";
-    f_code := (
-      <[ "#0" :=
-        locinfo: loc_37 ;
-        "_" <- LocInfoE loc_61 (sl_lock) with
-          [ LocInfoE loc_62 (&(LocInfoE loc_63 (lock))) ] ;
-        locinfo: loc_38 ;
-        annot: (UnlockA) ;
-        expr: (LocInfoE loc_58 (&(LocInfoE loc_59 (data)))) ;
-        locinfo: loc_49 ;
-        "$0" <- LocInfoE loc_51 (alloc) with
-          [ LocInfoE loc_52 (&(LocInfoE loc_53 (data))) ;
-          LocInfoE loc_54 (use{it_layout size_t} (LocInfoE loc_55 ("size"))) ] ;
-        "ret" <-{ LPtr } LocInfoE loc_49 ("$0") ;
-        locinfo: loc_41 ;
-        "_" <- LocInfoE loc_46 (sl_unlock) with
-          [ LocInfoE loc_47 (AnnotExpr 1%nat LockA (LocInfoE loc_47 (&(LocInfoE loc_48 (lock))))) ] ;
-        locinfo: loc_42 ;
-        Return (LocInfoE loc_43 (use{LPtr} (LocInfoE loc_44 ("ret"))))
       ]> $∅
     )%E
   |}.
@@ -268,59 +236,90 @@ Section code.
     f_code := (
       <[ "#0" :=
         "cur" <-{ LPtr }
-          LocInfoE loc_123 (use{LPtr} (LocInfoE loc_124 ("list"))) ;
-        locinfo: loc_67 ;
+          LocInfoE loc_93 (use{LPtr} (LocInfoE loc_94 ("list"))) ;
+        locinfo: loc_37 ;
         Goto "#1"
       ]> $
       <[ "#1" :=
-        locinfo: loc_117 ;
-        if: LocInfoE loc_117 (UnOp (CastOp $ IntOp bool_it) (IntOp i32) (LocInfoE loc_117 ((LocInfoE loc_118 (use{LPtr} (LocInfoE loc_120 (!{LPtr} (LocInfoE loc_121 ("cur")))))) !={PtrOp, PtrOp} (LocInfoE loc_122 (NULL)))))
+        locinfo: loc_87 ;
+        if: LocInfoE loc_87 (UnOp (CastOp $ IntOp bool_it) (IntOp i32) (LocInfoE loc_87 ((LocInfoE loc_88 (use{LPtr} (LocInfoE loc_90 (!{LPtr} (LocInfoE loc_91 ("cur")))))) !={PtrOp, PtrOp} (LocInfoE loc_92 (NULL)))))
         then
-        locinfo: loc_108 ;
+        locinfo: loc_78 ;
           Goto "#2"
         else
         Goto "#3"
       ]> $
       <[ "#2" :=
-        locinfo: loc_108 ;
-        if: LocInfoE loc_108 (UnOp (CastOp $ IntOp bool_it) (IntOp i32) (LocInfoE loc_108 ((LocInfoE loc_109 (use{it_layout size_t} (LocInfoE loc_110 ("size")))) ≤{IntOp size_t, IntOp size_t} (LocInfoE loc_111 (use{it_layout size_t} (LocInfoE loc_112 ((LocInfoE loc_113 (!{LPtr} (LocInfoE loc_115 (!{LPtr} (LocInfoE loc_116 ("cur")))))) at{struct_chunk} "size")))))))
+        locinfo: loc_78 ;
+        if: LocInfoE loc_78 (UnOp (CastOp $ IntOp bool_it) (IntOp i32) (LocInfoE loc_78 ((LocInfoE loc_79 (use{it_layout size_t} (LocInfoE loc_80 ("size")))) ≤{IntOp size_t, IntOp size_t} (LocInfoE loc_81 (use{it_layout size_t} (LocInfoE loc_82 ((LocInfoE loc_83 (!{LPtr} (LocInfoE loc_85 (!{LPtr} (LocInfoE loc_86 ("cur")))))) at{struct_chunk} "size")))))))
         then
         Goto "#5"
         else
-        locinfo: loc_96 ;
+        locinfo: loc_66 ;
           Goto "#6"
       ]> $
       <[ "#3" :=
         "entry" <-{ LPtr }
-          LocInfoE loc_89 (UnOp (CastOp $ PtrOp) (PtrOp) (LocInfoE loc_89 (use{LPtr} (LocInfoE loc_90 ("data"))))) ;
-        locinfo: loc_69 ;
-        LocInfoE loc_84 ((LocInfoE loc_85 (!{LPtr} (LocInfoE loc_86 ("entry")))) at{struct_chunk} "size") <-{ it_layout size_t }
-          LocInfoE loc_87 (use{it_layout size_t} (LocInfoE loc_88 ("size"))) ;
-        locinfo: loc_70 ;
-        LocInfoE loc_77 ((LocInfoE loc_78 (!{LPtr} (LocInfoE loc_79 ("entry")))) at{struct_chunk} "next") <-{ LPtr }
-          LocInfoE loc_80 (use{LPtr} (LocInfoE loc_82 (!{LPtr} (LocInfoE loc_83 ("cur"))))) ;
-        locinfo: loc_71 ;
-        LocInfoE loc_73 (!{LPtr} (LocInfoE loc_74 ("cur"))) <-{ LPtr }
-          LocInfoE loc_75 (use{LPtr} (LocInfoE loc_76 ("entry"))) ;
+          LocInfoE loc_59 (UnOp (CastOp $ PtrOp) (PtrOp) (LocInfoE loc_59 (use{LPtr} (LocInfoE loc_60 ("data"))))) ;
+        locinfo: loc_39 ;
+        LocInfoE loc_54 ((LocInfoE loc_55 (!{LPtr} (LocInfoE loc_56 ("entry")))) at{struct_chunk} "size") <-{ it_layout size_t }
+          LocInfoE loc_57 (use{it_layout size_t} (LocInfoE loc_58 ("size"))) ;
+        locinfo: loc_40 ;
+        LocInfoE loc_47 ((LocInfoE loc_48 (!{LPtr} (LocInfoE loc_49 ("entry")))) at{struct_chunk} "next") <-{ LPtr }
+          LocInfoE loc_50 (use{LPtr} (LocInfoE loc_52 (!{LPtr} (LocInfoE loc_53 ("cur"))))) ;
+        locinfo: loc_41 ;
+        LocInfoE loc_43 (!{LPtr} (LocInfoE loc_44 ("cur"))) <-{ LPtr }
+          LocInfoE loc_45 (use{LPtr} (LocInfoE loc_46 ("entry"))) ;
         Return (VOID)
       ]> $
       <[ "#4" :=
-        locinfo: loc_96 ;
-        LocInfoE loc_99 ("cur") <-{ LPtr }
-          LocInfoE loc_100 (&(LocInfoE loc_101 ((LocInfoE loc_102 (!{LPtr} (LocInfoE loc_104 (!{LPtr} (LocInfoE loc_105 ("cur")))))) at{struct_chunk} "next"))) ;
-        locinfo: loc_97 ;
-        Goto "continue7"
+        locinfo: loc_66 ;
+        LocInfoE loc_69 ("cur") <-{ LPtr }
+          LocInfoE loc_70 (&(LocInfoE loc_71 ((LocInfoE loc_72 (!{LPtr} (LocInfoE loc_74 (!{LPtr} (LocInfoE loc_75 ("cur")))))) at{struct_chunk} "next"))) ;
+        locinfo: loc_67 ;
+        Goto "continue4"
       ]> $
       <[ "#5" :=
         Goto "#3"
       ]> $
       <[ "#6" :=
-        locinfo: loc_96 ;
+        locinfo: loc_66 ;
         Goto "#4"
       ]> $
-      <[ "continue7" :=
-        locinfo: loc_67 ;
+      <[ "continue4" :=
+        locinfo: loc_37 ;
         Goto "#1"
+      ]> $∅
+    )%E
+  |}.
+
+  (* Definition of function [thread_safe_alloc]. *)
+  Definition impl_thread_safe_alloc (data lock alloc sl_lock sl_unlock : loc): function := {|
+    f_args := [
+      ("size", it_layout size_t)
+    ];
+    f_local_vars := [
+      ("ret", LPtr)
+    ];
+    f_init := "#0";
+    f_code := (
+      <[ "#0" :=
+        locinfo: loc_99 ;
+        "_" <- LocInfoE loc_123 (sl_lock) with
+          [ LocInfoE loc_124 (&(LocInfoE loc_125 (lock))) ] ;
+        locinfo: loc_100 ;
+        annot: (UnlockA) ;
+        expr: (LocInfoE loc_120 (&(LocInfoE loc_121 (data)))) ;
+        locinfo: loc_111 ;
+        "$0" <- LocInfoE loc_113 (alloc) with
+          [ LocInfoE loc_114 (&(LocInfoE loc_115 (data))) ;
+          LocInfoE loc_116 (use{it_layout size_t} (LocInfoE loc_117 ("size"))) ] ;
+        "ret" <-{ LPtr } LocInfoE loc_111 ("$0") ;
+        locinfo: loc_103 ;
+        "_" <- LocInfoE loc_108 (sl_unlock) with
+          [ LocInfoE loc_109 (AnnotExpr 1%nat LockA (LocInfoE loc_109 (&(LocInfoE loc_110 (lock))))) ] ;
+        locinfo: loc_104 ;
+        Return (LocInfoE loc_105 (use{LPtr} (LocInfoE loc_106 ("ret"))))
       ]> $∅
     )%E
   |}.
@@ -336,9 +335,9 @@ Section code.
     f_init := "#0";
     f_code := (
       <[ "#0" :=
-        locinfo: loc_129 ;
-        "_" <- LocInfoE loc_131 (use{LPtr} (LocInfoE loc_132 ("fn"))) with
-          [ LocInfoE loc_133 (use{LPtr} (LocInfoE loc_134 ("arg"))) ] ;
+        locinfo: loc_128 ;
+        "_" <- LocInfoE loc_130 (use{LPtr} (LocInfoE loc_131 ("fn"))) with
+          [ LocInfoE loc_132 (use{LPtr} (LocInfoE loc_133 ("arg"))) ] ;
         Return (VOID)
       ]> $∅
     )%E
@@ -356,10 +355,10 @@ Section code.
     f_code := (
       <[ "#0" :=
         "num_int" <-{ LPtr }
-          LocInfoE loc_145 (UnOp (CastOp $ PtrOp) (PtrOp) (LocInfoE loc_145 (use{LPtr} (LocInfoE loc_146 ("num"))))) ;
-        locinfo: loc_138 ;
-        "_" <- LocInfoE loc_140 (thread_safe_alloc) with
-          [ LocInfoE loc_141 (use{it_layout size_t} (LocInfoE loc_143 (!{LPtr} (LocInfoE loc_144 ("num_int"))))) ] ;
+          LocInfoE loc_144 (UnOp (CastOp $ PtrOp) (PtrOp) (LocInfoE loc_144 (use{LPtr} (LocInfoE loc_145 ("num"))))) ;
+        locinfo: loc_137 ;
+        "_" <- LocInfoE loc_139 (thread_safe_alloc) with
+          [ LocInfoE loc_140 (use{it_layout size_t} (LocInfoE loc_142 (!{LPtr} (LocInfoE loc_143 ("num_int"))))) ] ;
         Return (VOID)
       ]> $∅
     )%E
@@ -374,16 +373,16 @@ Section code.
     f_init := "#0";
     f_code := (
       <[ "#0" :=
+        locinfo: loc_150 ;
+        LocInfoE loc_161 (param) <-{ it_layout size_t }
+          LocInfoE loc_162 (UnOp (CastOp $ IntOp size_t) (IntOp i32) (LocInfoE loc_162 (i2v 5 i32))) ;
         locinfo: loc_151 ;
-        LocInfoE loc_162 (param) <-{ it_layout size_t }
-          LocInfoE loc_163 (UnOp (CastOp $ IntOp size_t) (IntOp i32) (LocInfoE loc_163 (i2v 5 i32))) ;
+        "_" <- LocInfoE loc_157 (fork) with
+          [ LocInfoE loc_158 (test_thread_safe_alloc_fork_fn) ;
+          LocInfoE loc_159 (&(LocInfoE loc_160 (param))) ] ;
         locinfo: loc_152 ;
-        "_" <- LocInfoE loc_158 (fork) with
-          [ LocInfoE loc_159 (test_thread_safe_alloc_fork_fn) ;
-          LocInfoE loc_160 (&(LocInfoE loc_161 (param))) ] ;
-        locinfo: loc_153 ;
-        "_" <- LocInfoE loc_155 (thread_safe_alloc) with
-          [ LocInfoE loc_156 (UnOp (CastOp $ IntOp size_t) (IntOp i32) (LocInfoE loc_156 (i2v 5 i32))) ] ;
+        "_" <- LocInfoE loc_154 (thread_safe_alloc) with
+          [ LocInfoE loc_155 (UnOp (CastOp $ IntOp size_t) (IntOp i32) (LocInfoE loc_155 (i2v 5 i32))) ] ;
         Return (VOID)
       ]> $∅
     )%E
