examples/proofs/paper_examples/generated_spec.v
@@ -8,51 +8,62 @@ Section spec.
   Context `{!typeG Σ} `{!globalG Σ}.
   Context `{!lockG Σ}.
 
-  (* Definition of type [alloc_data]. *)
-  Definition alloc_data_rec : (nat -d> typeO) → (nat -d> typeO) := (λ self nlen,
-    struct struct_alloc_data [@{type}
-      (nlen @ (int (size_t))) ;
-      (&own (uninit (ly_set_size u8 nlen)))
+  (* Inlined code. *)
+
+  Notation "P ? l : r" :=
+    (if bool_decide P then l else r)
+    (at level 100, l at next level, r at next level).
+
+  Close Scope Z.
+
+  Definition byte_layout : nat → layout := ly_set_size u8.
+  Coercion byte_layout : nat >-> layout.
+
+  (* Definition of type [mem_t]. *)
+  Definition mem_t_rec : (nat -d> typeO) → (nat -d> typeO) := (λ self a,
+    struct struct_mem_t [@{type}
+      (a @ (int (size_t))) ;
+      (&own (uninit (a)))
     ]
   )%I.
-  Typeclasses Opaque alloc_data_rec.
+  Typeclasses Opaque mem_t_rec.
 
-  Global Instance alloc_data_rec_ne : Contractive alloc_data_rec.
+  Global Instance mem_t_rec_ne : Contractive mem_t_rec.
   Proof. solve_type_proper. Qed.
 
-  Definition alloc_data : rtype := {|
+  Definition mem_t : rtype := {|
     rty_type := nat;
-    rty r__ := fixp alloc_data_rec r__
+    rty r__ := fixp mem_t_rec r__
   |}.
 
-  Lemma alloc_data_unfold (nlen : nat) :
-    (nlen @ alloc_data)%I ≡@{type} (
-      struct struct_alloc_data [@{type}
-        (nlen @ (int (size_t))) ;
-        (&own (uninit (ly_set_size u8 nlen)))
+  Lemma mem_t_unfold (a : nat) :
+    (a @ mem_t)%I ≡@{type} (
+      struct struct_mem_t [@{type}
+        (a @ (int (size_t))) ;
+        (&own (uninit (a)))
       ]
     )%I.
   Proof. by rewrite {1}/with_refinement/=fixp_unfold. Qed.
 
 
-  Global Program Instance alloc_data_rmovable : RMovable alloc_data :=
-    {| rmovable 'nlen := movable_eq _ _ (alloc_data_unfold nlen) |}.
+  Global Program Instance mem_t_rmovable : RMovable mem_t :=
+    {| rmovable 'a := movable_eq _ _ (mem_t_unfold a) |}.
   Next Obligation. solve_ty_layout_eq. Qed.
 
-  Global Instance alloc_data_simplify_hyp_place_inst l_ β_ (nlen : nat) :
-    SimplifyHypPlace l_ β_ (nlen @ alloc_data)%I (Some 100%N) :=
-    λ T, i2p (simplify_hyp_place_eq l_ β_ _ _ T (alloc_data_unfold _)).
-  Global Instance alloc_data_simplify_goal_place_inst l_ β_ (nlen : nat) :
-    SimplifyGoalPlace l_ β_ (nlen @ alloc_data)%I (Some 100%N) :=
-    λ T, i2p (simplify_goal_place_eq l_ β_ _ _ T (alloc_data_unfold _)).
+  Global Instance mem_t_simplify_hyp_place_inst l_ β_ (a : nat) :
+    SimplifyHypPlace l_ β_ (a @ mem_t)%I (Some 100%N) :=
+    λ T, i2p (simplify_hyp_place_eq l_ β_ _ _ T (mem_t_unfold _)).
+  Global Instance mem_t_simplify_goal_place_inst l_ β_ (a : nat) :
+    SimplifyGoalPlace l_ β_ (a @ mem_t)%I (Some 100%N) :=
+    λ T, i2p (simplify_goal_place_eq l_ β_ _ _ T (mem_t_unfold _)).
 
-  Global Program Instance alloc_data_simplify_hyp_val_inst v_ (nlen : nat) :
-    SimplifyHypVal v_ (nlen @ alloc_data)%I (Some 100%N) :=
-    λ T, i2p (simplify_hyp_val_eq v_ _ _ (alloc_data_unfold _) T _).
+  Global Program Instance mem_t_simplify_hyp_val_inst v_ (a : nat) :
+    SimplifyHypVal v_ (a @ mem_t)%I (Some 100%N) :=
+    λ T, i2p (simplify_hyp_val_eq v_ _ _ (mem_t_unfold _) T _).
   Next Obligation. done. Qed.
-  Global Program Instance alloc_data_simplify_goal_val_inst v_ (nlen : nat) :
-    SimplifyGoalVal v_ (nlen @ alloc_data)%I (Some 100%N) :=
-    λ T, i2p (simplify_goal_val_eq v_ _ _ (alloc_data_unfold _) T _).
+  Global Program Instance mem_t_simplify_goal_val_inst v_ (a : nat) :
+    SimplifyGoalVal v_ (a @ mem_t)%I (Some 100%N) :=
+    λ T, i2p (simplify_goal_val_eq v_ _ _ (mem_t_unfold _) T _).
   Next Obligation. done. Qed.
 
   (* Definition of type [chunks_t]. *)
@@ -139,19 +150,19 @@ Section spec.
 
   (* Specifications for function [alloc]. *)
   Definition type_of_alloc :=
-    fn(∀ (nlen, nsize, p) : nat * nat * loc; (p @ (&own (nlen @ (alloc_data)))), (nsize @ (int (size_t))); True)
-      → ∃ () : (), ((nsize <= nlen) @ (optional (&own (uninit (ly_set_size u8 nsize))) (null))); (p ◁ₗ ((if bool_decide(nsize <= nlen) then (nlen - nsize)%nat else nlen) @ (alloc_data))).
-
-  (* Specifications for function [thread_safe_alloc]. *)
-  Definition type_of_thread_safe_alloc :=
-    fn(∀ (lid, nsize) : lock_id * nat; (nsize @ (int (size_t))); (initialized "lock" lid) ∗ (initialized "data" lid))
-      → ∃ () : (), (optionalO (λ _ : unit,
-        &own (uninit (ly_set_size u8 nsize)) ) (null)); True.
+    fn(∀ (a, n, p) : nat * nat * loc; (p @ (&own (a @ (mem_t)))), (n @ (int (size_t))); True)
+      → ∃ () : (), ((n ≤ a) @ (optional (&own (uninit (n))) (null))); (p ◁ₗ ((n ≤ a ? a - n : a) @ (mem_t))).
 
   (* Specifications for function [free]. *)
   Definition type_of_free :=
     fn(∀ (s, p, ly) : (gmultiset layout) * loc * layout; (p @ (&own (s @ (chunks_t)))), (&own (uninit (ly))), ((ly.(ly_size)) @ (int (size_t))); ⌜layout_of struct_chunk ⊑ ly⌝)
       → ∃ () : (), (void); (p ◁ₗ (({[ly]} ⊎ s) @ (chunks_t))).
+
+  (* Specifications for function [thread_safe_alloc]. *)
+  Definition type_of_thread_safe_alloc :=
+    fn(∀ (lid, n) : lock_id * nat; (n @ (int (size_t))); (initialized "lock" lid) ∗ (initialized "data" lid))
+      → ∃ () : (), (optionalO (λ _ : unit,   &own (uninit (n))
+      ) (null)); True.
 
   (* Specifications for function [fork]. *)
   Definition type_of_fork :=
@@ -169,5 +180,5 @@ Section spec.
       → ∃ () : (), (void); True.
 End spec.
 
-Typeclasses Opaque alloc_data_rec.
+Typeclasses Opaque mem_t_rec.
 Typeclasses Opaque chunks_t_rec.
