examples/proofs/paper_examples/generated_proof_thread_safe_alloc.v
@@ -13,14 +13,14 @@ Section proof_thread_safe_alloc.
   Lemma type_thread_safe_alloc (data lock alloc sl_lock sl_unlock : loc) :
     global_locs !! "data" = Some data →
     global_locs !! "lock" = Some lock →
-    global_initialized_types !! "data" = Some (GT lock_id (λ 'lid, (spinlocked (lid) ("data") (alloc_data)) : type)) →
+    global_initialized_types !! "data" = Some (GT lock_id (λ 'lid, (spinlocked (lid) ("data") (mem_t)) : type)) →
     global_initialized_types !! "lock" = Some (GT lock_id (λ 'lid, (spinlock (lid)) : type)) →
     alloc ◁ᵥ alloc @ function_ptr type_of_alloc -∗
     sl_lock ◁ᵥ sl_lock @ function_ptr type_of_sl_lock -∗
     sl_unlock ◁ᵥ sl_unlock @ function_ptr type_of_sl_unlock -∗
     typed_function (impl_thread_safe_alloc data lock alloc sl_lock sl_unlock) type_of_thread_safe_alloc.
   Proof.
-    start_function "thread_safe_alloc" ([lid nsize]) => arg_size local_ret.
+    start_function "thread_safe_alloc" ([lid n]) => arg_size local_ret.
     split_blocks ((
       ∅
     )%I : gmap label (iProp Σ)) ((
